fix: ensure the alive test cases still work after introducing a memory state

SSA/Projects/SLLVM/Dialect/Semantics/EffectM.lean
@@ -9,6 +9,7 @@ namespace LeanMLIR
 
 structure MemoryState where
   -- TODO: actually implement memory state
+  deriving Inhabited
 
 instance : Refinement MemoryState := .ofEq
 
@@ -19,6 +20,18 @@ namespace EffectM
 /-! ## Constructors -/
 
 abbrev ub : EffectM α := PoisonOr.poison
-abbrev value (a : α) : EffectM α := pure a
+abbrev value (a : α) : EffectM α := StateT.lift (PoisonOr.value a)
 
--- theorem pure_eq : pure
+@[simp, simp_denote]
+theorem pure_eq : @pure EffectM _ = @value := rfl
+
+@[simp, simp_denote]
+theorem lift_isRefinedBy_lift_iff [HRefinement α α] (a b : PoisonOr α) :
+    (StateT.lift a : EffectM α) ⊑ (StateT.lift b : EffectM α) ↔ a ⊑ b := by
+  rw [StateT.isRefinedBy_iff]
+  unfold StateT.lift
+  cases a; simp [-EffectKind.return_impure_toMonad_eq] -- TODO: this lemma causes an infinite loop
+  cases b; simp [-EffectKind.return_impure_toMonad_eq]
+
+  have (s : MemoryState) : s ⊑ s := by rfl
+  simp [-EffectKind.return_impure_toMonad_eq, this]
